src/michocott/michelson_tests.v
@@ -7,69 +7,82 @@ Import ListNotations.
 Hint Constructors BigStep.
 
 (* Notation for sequence of instructinos *)
-Notation "x ;; y" :=  (i_Seq x y) (at level 100)  : list_scope .
+Notation "x ;; y" :=  (i_SEQ x y) (at level 100)  : list_scope .
+
+(* Shortcuts for instructions *)
+Definition PUSH t x := (i_Fun (i_Non_failing (i_nff_nullary (i_PUSH t x)))).
+Definition ADD := (i_Fun i_ADD).
+Definition SUB := (i_Fun i_SUB).
+Definition DUP := (i_Fun (i_Non_failing (i_DUP))).
+Definition DIP c := i_DIP c.
+Definition SWAP := (i_Fun (i_Non_failing (i_SWAP))).
+Definition NEQ := (i_Fun (i_Non_failing (i_nff_unary (i_unary_comparison NEQ)))).
+Definition LOOP body := (i_LOOP body).
+Definition DROP := (i_Fun (i_Non_failing i_DROP)).
+Definition NIL ty := (i_Fun (i_Non_failing (i_nff_nullary (i_NIL ty)))). 
+Definition CONS := (i_Fun (i_Non_failing (i_nff_binary i_CONS))).
 
 Fact can_push94 :
-  (BigStep (i_Push (t_Ct ct_Nat) (d_Num (N_NatConstant 4)) ;;
-            i_Push (t_Ct ct_Nat) (d_Num (N_NatConstant 9)))
+  (BigStep (PUSH (ty_Comparable_type cty_nat) (d_Num (num_NatConstant 4)) ;;
+            PUSH (ty_Comparable_type cty_nat) (d_Num (num_NatConstant 9)))
            (SE_Stack [])
-           (SE_Stack [ (d_Num (N_NatConstant 9)) ; (d_Num (N_NatConstant 4)) ]) ).
+           (SE_Stack [ (d_Num (num_NatConstant 9)) ; (d_Num (num_NatConstant 4)) ]) ).
 Proof. repeat econstructor. Qed.
 
 
 Fact test_add :
-  (BigStep (i_Push (t_Ct ct_Nat) (d_Num (N_NatConstant 4)) ;;
-            i_Push (t_Ct ct_Nat) (d_Num (N_NatConstant 9)) ;;
-            i_Add)
+  (BigStep (PUSH (ty_Comparable_type cty_nat) (d_Num (num_NatConstant 4)) ;;
+            PUSH (ty_Comparable_type cty_nat) (d_Num (num_NatConstant 9)) ;;
+            ADD)
            (SE_Stack [])
-           (SE_Stack [ (d_Num (N_NatConstant 13)) ]) ).
+           (SE_Stack [ (d_Num (num_NatConstant 13)) ]) ).
 Proof. repeat econstructor. Qed.
 
 (* a less trivial example *)
 Definition fib (n : Z) :=
   (* push 1 1 on stack *)
-  i_Push (t_Ct ct_Nat) (d_Num (N_NatConstant 1)) ;;
-  i_Dup ;;
+  PUSH (ty_Comparable_type cty_nat) (d_Num (num_NatConstant 1)) ;;
+  DUP ;;
   (* push n on stack *)
-  i_Push (t_Ct ct_Int) (d_Num (N_IntConstant n)) ;;
+  PUSH (ty_Comparable_type cty_int) (d_Num (num_IntConstant n)) ;;
   (* push True *)
-  i_Push (t_Ct ct_Nat) (d_BoolConstant true) ;;
+  PUSH (ty_Comparable_type cty_nat) (d_Bool true) ;;
   (* stack := True ; n ; 1 1 *)
-  i_Loop (
+  LOOP (
       (* stack := n ; a ; b *)
-      i_Dip (
-          i_Dip ( i_Dup )  ;;
+      DIP (
+          DIP ( DUP )  ;;
           (* stack := n ; a ; b ; b *)
-          i_Dup ;;
+          DUP ;;
           (* stack := n ; a ; a ; b ; b *)
-          i_Dip ( i_Swap ) ;;
+          DIP ( SWAP ) ;;
           (* stack := n ; a ; b ; a ; b *)
-          i_Add
+          ADD
           (* stack := n ; a + b ; a ; b *)
       ) ;;
-      i_Push (t_Ct ct_Nat) (d_Num (N_NatConstant 1)) ;;
+      PUSH (ty_Comparable_type cty_nat) (d_Num (num_NatConstant 1)) ;;
       (* stack := 1 ; (n) ; a + b ; a ; b *)
-      i_Swap ;;
-      i_Sub ;;
+      SWAP ;;
+      SUB ;;
       (* stack := (n-1) ; a + b ; a ; b *)
 
-      i_Dup ;; i_Neq
+      DUP ;; NEQ
       (* stack := (n<>0) ; n ; a + b ; a ; b *)
   ) ;;
   (* stack := 0 ; fib n ; fib (n-1) ; ... *)
-  i_Drop.
+  DROP.
   (* stack := (fib (n+2)) ; fib (n+1) ; ... *)
 
 
 
-Definition fib5 := [ (d_Num (N_NatConstant 5)) ;
-                       (d_Num (N_NatConstant 3)) ;
-                       (d_Num (N_NatConstant 2)) ;
-                       (d_Num (N_NatConstant 1)) ;
-                       (d_Num (N_NatConstant 1)) ].
-Definition fib3 := [ (d_Num (N_NatConstant 2)) ;
-                       (d_Num (N_NatConstant 1)) ;
-                       (d_Num (N_NatConstant 1)) ].
+Definition fib5 := [ (d_Num (num_NatConstant 5)) ;
+                       (d_Num (num_NatConstant 3)) ;
+                       (d_Num (num_NatConstant 2)) ;
+                       (d_Num (num_NatConstant 1)) ;
+                       (d_Num (num_NatConstant 1)) ].
+Definition fib3 := [ (d_Num (num_NatConstant 2)) ;
+                       (d_Num (num_NatConstant 1)) ;
+                       (d_Num (num_NatConstant 1)) ].
 
 Fact test_fib3 :
   (BigStep (fib 1) (SE_Stack []) (SE_Stack fib3)).
@@ -84,24 +97,24 @@ Qed.
 
 (* Demonstrates how a ill typed program can be executed *)
 Definition c_ill_typed :=
-  i_Nil (t_Ct ct_Int) ;;
-  i_Push (t_Ct ct_Int) (d_Num (N_IntConstant 4)) ;;
-  i_Cons ;;
-  i_Push (t_Ct ct_Bool) (d_BoolConstant true) ;;
-  i_Cons.
+  NIL (ty_Comparable_type cty_int) ;;
+  PUSH (ty_Comparable_type cty_int) (d_Num (num_IntConstant 4)) ;;
+  CONS ;;
+  PUSH (ty_Comparable_type cty_bool) (d_Bool true) ;;
+  CONS.
 
 Fact ill_typed :
   (BigStep c_ill_typed
            (SE_Stack [])
-           (SE_Stack [ d_DataList [ d_BoolConstant true ; d_Num (N_IntConstant 4) ] ]) ).
+           (SE_Stack [ d_SetList [ d_Bool true ; d_Num (num_IntConstant 4) ] ]) ).
 Proof. repeat econstructor. Qed.
 
 
 (* Demonstrates how a ill typed program without semantics *)
 Definition c_ill_typed2 :=
-  i_Push (t_Ct ct_Int) (d_Num (N_IntConstant 4)) ;;
-  i_Push (t_Ct ct_Bool) (d_BoolConstant true) ;;
-  i_Add.
+  PUSH (ty_Comparable_type cty_int) (d_Num (num_IntConstant 4)) ;;
+  PUSH (ty_Comparable_type cty_bool) (d_Bool true) ;;
+  ADD.
 
 Fact ill_typed2 :
   ~ exists s, (BigStep c_ill_typed2
