src/michocott/Formulas.v
@@ -1,32 +1,26 @@
-Definition typeof (d : data) : type := t_Key.
+Definition typeof (d : data) : type := ty_key.
 
-(* 
- * Definition num_compat (d d' : num) : Prop :=
- *   typeof (d_Num d) = typeof (d_Num d').
- * 
- * Definition num_compat (d d' : num) : Prop :=
- *   typeof (d_Num d) = typeof (d_Num d').
- *)
-
+Definition num_compat (d d' : num) : Prop :=
+  typeof (d_Num d) = typeof (d_Num d').
 
 Definition lift_num (rn : nat -> nat -> Prop) (rz : Z -> Z -> Prop) : num -> num -> Prop :=
   fun N1 N2 =>
     match N1, N2 with
-      | N_IntConstant z1, N_IntConstant z2 => rz z1 z2
-      | N_NatConstant n1, N_NatConstant n2 => rn n1 n2
+      | num_IntConstant z1, num_IntConstant z2 => rz z1 z2
+      | num_NatConstant n1, num_NatConstant n2 => rn n1 n2
       | _, _ => False
     end.
 
 Definition lift_num2 (r : forall (A : Type) (_ _ : A), Prop) : (num -> num -> Prop) := lift_num (@r nat) (@r Z).
 
 
-Definition fun_lift_num (rn : nat -> nat -> nat) (rz : Z -> Z -> Z) : num -> num -> option num :=
-  fun N1 N2 =>
-    match N1, N2 with
-      | N_IntConstant z1, N_IntConstant z2 => Some (N_IntConstant (rz z1 z2))
-      | N_NatConstant n1, N_NatConstant n2 => Some (N_NatConstant (rn n1 n2))
-      | _, _ => None
-    end.
+(* Definition fun_lift_num (rn : nat -> nat -> nat) (rz : Z -> Z -> Z) : num -> num -> option num := *)
+(*   fun N1 N2 => *)
+(*     match N1, N2 with *)
+(*       | num_IntConstant z1, num_IntConstant z2 => Some (num_IntConstant (rz z1 z2)) *)
+(*       | num_NatConstant n1, num_NatConstant n2 => Some (num_NatConstant (rn n1 n2)) *)
+(*       | _, _ => None *)
+(*     end. *)
 
 (* 
  * Definition zaop (op : aop) : (Z -> Z -> Z) :=
@@ -58,22 +52,22 @@ Definition num_apply_aop (op : aop) (N1 N2 : num) :=
   match op with
   | aop_Add =>
     match N1, N2 with
-    | N_IntConstant z1, N_IntConstant z2 => N_IntConstant (Z.add z1 z2)
-    | N_IntConstant z1, N_NatConstant n2 => N_IntConstant (Z.add z1 (Z.of_nat n2))
-    | N_NatConstant n1, N_IntConstant z2 => N_IntConstant (Z.add (Z.of_nat n1) z2)
-    | N_NatConstant n1, N_NatConstant n2 => N_NatConstant (Nat.add n1 n2)
+    | num_IntConstant z1, num_IntConstant z2 => num_IntConstant (Z.add z1 z2)
+    | num_IntConstant z1, num_NatConstant n2 => num_IntConstant (Z.add z1 (Z.of_nat n2))
+    | num_NatConstant n1, num_IntConstant z2 => num_IntConstant (Z.add (Z.of_nat n1) z2)
+    | num_NatConstant n1, num_NatConstant n2 => num_NatConstant (Nat.add n1 n2)
     end
   | aop_Mul => match N1, N2 with
-    | N_IntConstant z1, N_IntConstant z2 => N_IntConstant (Z.mul z1 z2)
-    | N_IntConstant z1, N_NatConstant n2 => N_IntConstant (Z.mul z1 (Z.of_nat n2))
-    | N_NatConstant n1, N_IntConstant z2 => N_IntConstant (Z.mul (Z.of_nat n1) z2)
-    | N_NatConstant n1, N_NatConstant n2 => N_NatConstant (Nat.mul n1 n2)
+    | num_IntConstant z1, num_IntConstant z2 => num_IntConstant (Z.mul z1 z2)
+    | num_IntConstant z1, num_NatConstant n2 => num_IntConstant (Z.mul z1 (Z.of_nat n2))
+    | num_NatConstant n1, num_IntConstant z2 => num_IntConstant (Z.mul (Z.of_nat n1) z2)
+    | num_NatConstant n1, num_NatConstant n2 => num_NatConstant (Nat.mul n1 n2)
     end
   | aop_Sub => match N1, N2 with
-    | N_IntConstant z1, N_IntConstant z2 => N_IntConstant (Z.sub z1 z2)
-    | N_IntConstant z1, N_NatConstant n2 => N_IntConstant (Z.sub z1 (Z.of_nat n2))
-    | N_NatConstant n1, N_IntConstant z2 => N_IntConstant (Z.sub (Z.of_nat n1) z2)
-    | N_NatConstant n1, N_NatConstant n2 => N_IntConstant (Z.sub (Z.of_nat n1) (Z.of_nat n2))
+    | num_IntConstant z1, num_IntConstant z2 => num_IntConstant (Z.sub z1 z2)
+    | num_IntConstant z1, num_NatConstant n2 => num_IntConstant (Z.sub z1 (Z.of_nat n2))
+    | num_NatConstant n1, num_IntConstant z2 => num_IntConstant (Z.sub (Z.of_nat n1) z2)
+    | num_NatConstant n1, num_NatConstant n2 => num_IntConstant (Z.sub (Z.of_nat n1) (Z.of_nat n2))
     end
   (* TODO! *)
   (* 
@@ -82,16 +76,16 @@ Definition num_apply_aop (op : aop) (N1 N2 : num) :=
    * | aop_Lsl => fun nat nat' => 0
    * | aop_Lsr => fun nat nat' => 0
    *)
-  | _ => N_NatConstant 0
+  | _ => num_NatConstant 0
   end.
 
 
 Definition num_apply_bitop (op : bitop) (N1 N2 : num) : num :=
   match op with
-  (* todo *)
-  | bitop_Or => N_NatConstant 0
-  | bitop_And => N_NatConstant 0
-  | bitop_Xor => N_NatConstant 0
+  (* TODO *)
+  | bitop_Or => num_NatConstant 0
+  | bitop_And => num_NatConstant 0
+  | bitop_Xor => num_NatConstant 0
   end.
 
 (* TODO *)
@@ -99,14 +93,14 @@ Definition num_bit_neg (N1 : num) : num := N1.
 
 Definition num_neq_zero (N : num) : Prop :=
   match N with
-  | N_IntConstant z1 => z1 <> (0 % Z)
-  | N_NatConstant n1 => n1 <> (0 % nat)
+  | num_IntConstant z1 => z1 <> (0 % Z)
+  | num_NatConstant n1 => n1 <> (0 % nat)
   end.
 
 Definition num_neg ( N : num ) : num :=
   match N with
-  | N_IntConstant z1 => N_IntConstant (- z1)
-  | N_NatConstant n1 => N_IntConstant (- (Z.of_nat n1))
+  | num_IntConstant z1 => num_IntConstant (- z1)
+  | num_NatConstant n1 => num_IntConstant (- (Z.of_nat n1))
   end.
 
 Definition TODO : Prop := False.
@@ -119,3 +113,26 @@ Definition TODO : Prop := False.
  *   | bop_Xor => xorb
  *   end.
  *)
+
+Definition compare x comp y :=
+    match x, y with
+    | d_Num (num_NatConstant x), d_Num (num_NatConstant y) =>
+         match comp with
+         | EQ => x = y
+         | NEQ => x <> y
+         | LT => x < y
+         | GT => x > y
+         | LE => x <= y
+         | GE => x >= y
+         end
+    | d_Num (num_IntConstant x), d_Num (num_IntConstant y) =>
+         match comp with
+         | EQ => Z.eq x y
+         | NEQ => x <> y
+         | LT => Z.lt x y
+         | GT => Z.gt x y
+         | LE => Z.le x y
+         | GE => Z.ge x y
+         end
+    | _,_ => False (* TODO *)
+    end.
